Volume 05 - Verifiable C. Verif sumarray (part 2)

Volume05-VerifiableC/Verif_sumarray.v
@@ -72,4 +72,324 @@ Proof.
 
 
 (* API Spec for the sumarray.c program
+
+   The Application Programmer Interface (API) of a C program is expressed in its
+   header file: function prototypes and data-structure definitions. In Verifiable C,
+   an API specification is written as a series of function specifications (`funspec`'s)
+   corresponding to the function prototypes.
+
+   This `DECLARE` statement has type `ident * funspec`. That is, it associates the name
+   of a function (the identifier `_sumarray`) with a function-specification. The identifier
+   `_sumarray` comes directly from the C program, as parsed by `clightgen`.
+
+   A function is specified by its precondition and its postcondition. The `WITH` clause
+   quantifies over Coq values that may appear in both the precondition and the postcondition.
+   The precondition has access to the function parameters (in this case `a` and `size`) and
+   the postcondition has access to the return value (`sum_Z contents`).
+
+   Function preconditions, postconditions, and loop invariants are assertions about the state
+   of variables and memory at a particular program point. In an assertion
+
+             PROP (P) LOCAL(Q) SEP (R)
+
+   the propositions in the sequence `P` are all of Coq type `Prop`. They describe things that
+   are true independent of program state. In the precondition above, the statement
+
+             0 <= size <= Int.max_signed
+
+   is true just within the scope of the quantification of the variable `size`; that variable
+   is bound by `WITH`, and spans the `PRE` and `POST` assertions.
+
+   The `LOCAL` clause, describing what's in C local variables, takes different forms depending
+   on context:
+
+      - In a function-precondition, we write PROP/PARAMS/SEP, that is, the PARAMS lists
+        the values of C function parameters (in order).
+      - In a function-postcondition, we write RETURN(v) to indicate the return value of
+        the function.
+      - Within a function body (in assertions and invariants) we write LOCAL to describe
+        the values of local variables (including parameters).
  *)
+Definition sumarray_spec : ident * funspec :=
+DECLARE _sumarray
+ WITH a : val, sh : share, contents : list Z, size : Z
+ PRE [ tptr tuint, tint ]
+  PROP (readable_share sh; 0 <= size <= Int.max_signed;
+         Forall (fun x => 0 <= x <= Int.max_unsigned) contents)
+  PARAMS (a; Vint (Int.repr size))
+  SEP (data_at sh (tarray tuint size) (map Vint (map Int.repr contents)) a)
+ POST [ tuint ]
+  PROP () RETURN (Vint (Int.repr (sum_Z contents)))
+  SEP (data_at sh (tarray tuint size) (map Vint (map Int.repr contents)) a).
+(* Whether it is PARAMS or RETURN or LOCAL, we are talking about the values contained in parameters
+  or local variables. In general, a C scalar variable holds something of type `val`; this type is
+  defined by CompCert as,
+ *)
+Print val.
+
+(* In an assertion `PROP(P) LOCAL(Q) SEP(R)`, the `SEP` conjuncts `R` are spatial assertions in
+   separation logic. In our example precondition, there's just one `SEP` conjunct, a `data_at`
+   assertion saying that at address `a` in memory, there is a data structure of type
+
+             array[size] of unsigned int;
+
+   with access-permission `sh`, and the contents of that array is the sequence
+
+             map Vint (map Int.repr contents)
+
+   The postcondition is introduced by `POST [ tuint ]`, indicating that this function returns a value
+   of type `unsigned int`. There are no `PROP` statements in this postcondition -- no forever-true facts
+   hold now, that weren't already true on entry to the function.
+
+   `RETURN(v)` gives the return value `v`; `RETURN()` for void functions.
+
+   The postcondition's `SEP` clause mentions all the spatial resources from the precondition, minus ones
+   that have been freed (deallocated), plus ones that have been malloc'd (allocated).
+
+   So, overall, the specification for sumarray is this: "At any call to sumarray, there exist values a, sh,
+   contents, size such that sh gives at least read-permission; `size` is representable as a nonnegative 32-bit
+   signed integer; function-parameter `_a` contains value `a` and `_n` contains the 32-bit representation of `size`;
+   and there's an array in memory at address `a` with permission `sh` containing contents. The function returns
+   a value equal to `sum_int(contents)`, and leaves the array in memory unaltered."
+ *)
+
+(* Function specification for main()
+
+   The function-spec for `main` has a special form.
+
+   This postcondition says we have indeed added up the global array `four`.
+ *)
+Definition main_spec :=
+ DECLARE _main
+  WITH gv : globals
+  PRE [] main_pre prog tt gv
+  POST [ tint ]
+     PROP()
+     RETURN (Vint (Int.repr (1+2+3+4)))
+     SEP(TT).
+
+(* Integer overflow
+
+   In Verifiable C's signed integer arithmetic, you must prove (if the system cannot prove automatically) that no
+   overflow occurs. For unsigned integers, arithmetic is treated as modulo-2^n (where n is typically 32 or 64),
+   and overflow is not an issue. The function Int.repr: Z → int truncates mathematical integers into 32-bit integers
+   by taking the (sign-extended) low-order 32 bits. Int.signed: int → Z injects back into the signed integers.
+
+   The sumarray program uses unsigned arithmetic for s and the array contents; it uses signed arithmetic for i.
+
+   The postcondition guarantees that the value returned is Int.repr (sum_Z contents). But what if the sum of all the
+   s is larger than 2^32, so the sum doesn't fit in a 32-bit signed integer? Then Int.unsigned(Int.repr (sum_Z contents))
+   ≠ sum_Z contents. In general, for a claim about Int.repr(x) to be useful one also needs to know that 0 ≤ x ≤ Int.max_unsigned
+   or Int.min_signed ≤ x ≤ Int.max_signed. The caller of sumarray will probably need to prove 0 ≤ sum_Z contents ≤ Int.max_unsigned
+   in order to make much use of the postcondition.
+ *)
+
+
+(* Packaging the Gprog and Vprog
+
+   To prove the correctness of a whole program,
+
+      - 1. Collect the function-API specs together into `Gprog`.
+      - 2. Prove that each function satisfies its own API spec (with a `semax_body` proof).
+      - 3. Tie everything together with a `semax_func` proof.
+
+   The first step is easy:
+ *)
+Definition Gprog := [sumarray_spec; main_spec].
+(* What's in Gprog are the funspecs that we built using DECLARE. (In multi-module programs we would also include imported funspecs.)
+
+   In addition to Gprog, the API spec contains Vprog, the list of global-variable type-specs. This was computed automatically by the
+   mk_varspecs tactic, in the "boilerplate" code above.
+ *)
+Print Vprog.         (*   = (_four, tarray tuint 4)  : varspecs *)
+Print varspecs.      (*   = list (ident * type) *)
+
+
+(* Proof of the sumarray program
+
+   Now comes the proof that f_sumarray, the body of the sumarray() function, satisfies sumarray_spec, in global context (Vprog,Gprog).
+
+   Here, `f_sumarray` is the actual function body (AST of the C code) as parsed by `clightgen`. We can read `body_sumarray` as claiming:
+   in the context of `Vprog` and `Gprog`, the function body `f_sumarray` satisfies its specification `sumarray_spec`. We need the context
+   in case the sumarray function refers to a global variable (`Vprog` provides the variable's type) or calls a globa function (`Gprog`
+   provides the function's API spec).
+
+ *)
+Lemma body_sumarray : semax_body Vprog Gprog f_sumarray sumarray_spec.
+Proof.
+  (** start function
+
+   The predicate [semax_body] states the Hoare triple of the function body,
+   [Delta |- {Pre} c {Post}], where [Pre] and [Post] are taken from the
+   [funspec], [c] is the body of the function, and the type-context [Delta]
+   is calculated from the global type-context overlaid with the parameter-
+   and local-types of the function.
+
+   To prove this, we begin with the tactic [start_function],  which takes care
+   of some simple bookkeeping and expresses the Hoare triple to be proved.
+   *)
+  start_function. (* always do this at the beginning of a `semax_body` proof *)
+
+  (** Some of the assumptions you now see above the line are,
+  - [a, sh, contents, size], taken directly from the WITH clause
+       of [sumarray_spec];
+  - [Delta_specs], the context in which Floyd's proof tactics will look up
+       the specifications of global functions;
+  - [Delta], the context in which Floyd will look up the types of
+       local and global variables;
+  - [SH,H,H0], taken exactly from the [PROP] clauses of [sumarray_spec]'s
+       precondition.
+
+  There are also two abbreviations above the line, POSTCONDITION and MORE_COMMANDS
+  *)
+
+  (** Forward symbolic execution
+
+  We do Hoare logic proof by forward symbolic execution.  At the beginning
+  of this function body, our proof goal is a Hoare triple about the statement
+  [(i=0; ...more commands...)]. In a forward Hoare logic proof of
+  [{P}(i=0;...more...){R}] we might first apply the sequence rule,
+
+    {P}(i=0;){Q}  {Q}(...more...){R}
+    ---------------------------------
+    {P}(i=0;...more...){R}
+
+  assuming we could derive some appropriate assertion [Q].
+  For many kinds of statements (assignments, return, break,
+  continue) [Q] is derived automatically by the [forward] tactic,
+  which applies a strongest-postcondition style of proof rule.
+  Let us now apply the [forward] tactic: *)
+  forward. (* i = 0; *)
+  (** Look at the precondition of the current proof goal, that is, the second
+   argument of `semax`; it has the form `PROP(...) LOCAL(...) SEP(...)`. That
+   precondition is also the postcondition of `i = 0;`. It's much like the
+   precondition of `i = 0;` except for one change: we now know that `i` is
+   equal to `0`, which is expressed in the `LOCAL` part as `temp _i (Vint (Int.repr 0))`
+  *)
+  Check 0.                              (* : Z, the mathematical integer zero *)
+  Check (Int.repr 0).                   (* : int, the 32-bit integer representing 0 *)
+  Check (Vint (Int.repr 0)).            (* : val, the type of CompCert values *)
+  Check (temp _i (Vint (Int.repr 0))).  (* : localdef, the type of `LOCAL` assertions *)
+
+  (** abbreviate, MORE_COMMANDS, POSTCONDITION
+
+   When doing forward symbolic execution (forward Floyd/Hoare proof) through a large function,
+   you don't usually want to see the entire function-body in your proof subgoal. Therefore the
+   system abbreviates some things for you, using the magic of Coq's implicit arguments.
+   *)
+  Check @abbreviate.      (* : forall A : Type, A -> A *)
+  About abbreviate.       (* Arguments A, x are implicit and maximally inserted ... *)
+  (* We see here that `abbreviate` is just the identity function, with both of its arguments
+   implicit.
+
+   To examinate the actual contents of `MORE_COMMANDS`, just do this:
+   *)
+  unfold abbreviate in MORE_COMMANDS.
+  (* or alternatively, *)
+
+  subst MORE_COMMANDS; unfold abbreviate.
+
+  (* Similarly, to see the `POSTCONDITION`, just do,
+   *)
+  unfold abbreviate in POSTCONDITION.
+
+  (* Hint
+
+   In any VST proof state, the [hint] tactic will print a suggestion (if it can) that will help
+   you make progress in the proof. In stepping through the case study in this chapter, insert
+   [hint] at any point to see what it says.
+   *)
+  hint.
+  (* Then delete the hints! (They slow down replay of your proof.)
+
+   The hint here suggests using `abbreviate_semax`, which will undo the [unfold abbreviate] that
+   we did above. Really this is optional; if we don't do [abbreviate_semax], the next [forward]
+   tactic will do it for us.
+   *)
+  abbreviate_semax.
+  hint.
+
+  (** Forward through another assignment statement
+
+   The [forward] tactic works on assignment statements, break, continue, and return.
+   *)
+  forward.  (* s = 0; *)
+
+  (** While loops, forward_while
+
+   To do symbolic execution through a `while` loop, use the [forward_while] tactic; you must
+   supply a loop invariant.
+
+   A loop invariant is an assertion, almost always in the form of an existential quantifier,
+
+            EX...PROP(...)LOCAL(...)SEP(...)
+
+   Each iteration of the loop has a state characterized by a different value of some iteration
+   variable(s), the EX binds that value.
+   *)
+  forward_while
+    (EX i: Z,
+      PROP (0 <= i <= size)
+      LOCAL (temp _a a;
+             temp _i (Vint (Int.repr i));
+             temp _n (Vint (Int.repr size));
+             temp _s (Vint (Int.repr (sum_Z (sublist 0 i contents)))))
+      SEP (data_at sh (tarray tuint size) (map Vint (map Int.repr contents)) a)).
+
+  (* [forward_while] leaves four subgoals; here we label them with the - bullet.
+
+   The first subgoal is to prove that the current assertion (precondition) entails the loop
+   invariant.
+   *)
+  - hint.
+
+  (** Proving separation-logic entailments
+
+   This proof goal is an entailment, [ENTAIL Delta, P |-- Q], meaning "in context `Delta`, any
+   state that satisfies `P` will also satisfy `Q`."
+
+   In this case, the right-hand-side of this entailment is existentially quantified; it says:
+   there exists a value `i` such that (among other things) `temp _i (Vint (Int.repr i))`, that
+   is, the C variable `_i` contains the value `i`. But the left-hand-side of the entailment
+   says `temp _i (Vint (Int.repr 0))`, that is, the C variable `_i` contains 0.
+
+   This is analogous to the following situation; and to prove such a goal, one uses Coq's "exists"
+   tactic to demonstrate a value for `i`.
+   *)
+  Set Nested Proofs Allowed.
+  Goal forall (f: Z -> Z) (x: Z), f(x)=0 -> exists i:Z, f(x) = i.
+    intros.
+    exists 0. auto. Qed.
+
+  (* In a separation logic entailment, one can prove an [EX] on the right-hand side by using the
+   [Exists] tactic to demonstrate a value for the quantified variable:
+   *)
+  Exists 0.     (* Instantiate the existential on the right-side of |-- *)
+  (* Notice that `i` has now been replaced with `0` on the right side.
+
+   To prove entailments, we usually use the [entailer!] tactic to simplify the entailment as much
+   as possible -- or in many cases, to prove it entirely.
+   *)
+  entailer!.
+
+  (** Type-checking the loop test
+
+   The second subgoal of [forward_while] is always to prove that the loop-test expression can
+   evaluate without crashing -- that is, all the variables it references exist and are initialized,
+   it doesn't divide by zero, et cetera.
+
+   We call this a "type-checking condition", the predicate `tc_expr`. In this case, it's the while-
+   loop test `i < n` that must execute, so we see `tc_expr Delta (!(_i < _n))` on the right-hand
+   side of the entailment.
+
+   Very often, these `tc_expr` goals solve automatically by `entailer!`.
+   *)
+  - hint.
+  entailer!.
+
+  (** Proving that the loop body preserves the loop invariant
+
+   
+   *)
+  - hint.
+
